\section{Tutorial A1.4 Set 1}

\begin{problem}
    The notation $(1 + D)^{[n]}(y)$ is used to denote \[y + \binom{n}{1} \der{y}{x} + \binom{n}{2} \der[2]{y}{x} + \dots + \der[n]{y}{x}.\] Show that \[(1 + D)^{[1]} \bs{(1 + D)^{[1]} (y)} = (1 + D)^{[2]} (y).\] Use an integrating factor to solve the differential equation \[(1 + D)^{[1]}(y) = x.\] Use your solution of this equation to solve the differential equation \[(1 + D)^{[2]}(y) = x.\]
\end{problem}
\begin{solution}
    \begin{align*}
        (1 + D)^{[1]} \bs{(1 + D)^{[1]} (y)} &= (1 + D)^{[1]} \bp{y + \der{y}{x}}\\
        &= \bp{y + \der{y}{x}} + \bp{\der{y}{x} + \der[2]{y}{x}}\\
        &= y + \binom{2}{1} \der{y}{x} + \der[2]{y}{x}\\
        &= (1 + D)^{[2]} (y).
    \end{align*}

    The differential equation $(1 + D)^{[1]}(y) = x$ can be expanded as \[\der{y}{x} + y = x.\] The integrating factor is $\e^{\int \d x} = \e^x$. Multiplying through by $\e^x$, we get \[\der{}{x} \bp{\e^x y} = \e^x \der{y}{x} + \e^x y = x \e^x.\] Hence, \[\e^x y = \int x \e^x \d x = \bp{x-1} \e^x + C.\] Thus, the general solution is \[y = x - 1 + C\e^{-x}.\]

    We have \[(1 + D)^{[2]}(y) = (1 + D)^{[1]} \bs{(1 + D)^{[1]} (y)} = x.\] Using the above solution, we see that \[(1 + D)^{[1]}(y) = x - 1 + C\e^{-x}.\] Once again, the integrating factor is $\e^x$. Multiplying it through yields \[\der{}{x} \bp{\e^x y} = x - 1 + C\e^{-x}.\] Thus, \[\e^x y = \int \bs{(x-1)\e^x + C} \d x = (x-2)\e^x + Cx + D.\] Hence, the general solution is \[y = x-2 + \bp{Cx + D} \e^{-x}.\]
\end{solution}

\begin{problem}
    \begin{enumerate}
        \item Use the substitution $y = v/t$ to reduce the differential equation \[2t^2 \der[2]{y}{t} + t\der{y}{t} - 3y = 0\] for $t > 0$ to \[2t\der[2]{v}{t} - 3\der{v}{t} = 0.\]
        \item Using a suitable substitution, show that the differential equation \[2t\der[2]{v}{t} - 3\der{v}{t} = 0\] can be reduced to \[2t \der{w}{t} - 3w = 0.\]
        \item Hence, find a general solution to the differential equation \[2t^2 \der[2]{y}{t} + t\der{y}{t} - 3y = 0.\]
    \end{enumerate}
\end{problem}
\begin{solution}
    \begin{ppart}
        Note that $y = v/t \implies v = yt$. Differentiating with respect to $t$, \[\der{v}{t} = t \der{y}{t} + y, \quad \der[2]{v}{t} = t\der[2]{y}{t} + 2 \der{y}{t}.\] Since \[2t^2 \der[2]{y}{t} + t\der{y}{t} - 3y = 2t \bp{t\der[2]{y}{t} + 2 \der{y}{t}} - 3\bp{t \der{y}{t} + y} = 0,\] we have \[2t\der[2]{v}{t} - 3\der{v}{t} = 0\] as desired.
    \end{ppart}
    \begin{ppart}
        Let $w = \derx{v}{t}$. Then the DE becomes \[2t \der{w}{t} - 3w = 0.\]
    \end{ppart}
    \begin{ppart}
        Note that the above DE can be written as \[\frac1w \der{w}{t} = \frac3{2t}.\] Integrating with respect to $t$, \[\ln \abs{w} + A = \frac32 \ln \abs{t} \implies w = B t^{3/2}.\] Hence, \[v = \int w \d t = \int B t^{3/2} \d t = C t^{5/2} + D.\] Finally, \[y = \frac{v}{t} = C t^{3/2} + D t^{-1}.\]
    \end{ppart}
\end{solution}