\section{Tutorial A1.4 Set 2}

\begin{problem}
    Reduce the differential equation \[\frac{x}{y} \der{y}{x} + \ln \frac{x^2}{y} = 2, \quad y > 0,\] to a differential equation in $x$ and $u$, where $u = y/x^2$. Hence, express $y$ in terms of $x$ and an arbitrary constant. Find the equation of the solution curve that passes through the point $(x, y) = (1, \e)$.
\end{problem}
\begin{solution}
    Note that $y = ux^2$. Differentiating with respect to $x$, we have \[\der{y}{x} = 2ux + x^2 \der{u}{x}.\] Substituting this into the given DE, we have \[\frac{x}{ux^2} \bp{2ux + x^2 \der{u}{x}} + \ln{\frac{x^2}{ux^2}} = 2,\] which simplifies to \[\frac1{u \ln u} \der{u}{x} = \frac1x.\] Integrating both sides with respect to $x$ yields $\ln \abs{\ln u} = \ln \abs{x} + A$, so $u = \e^{Bx}$ and thus $y = x^2 \e^{Bx}$. At $(x, y) = (1, \e)$, we have $\e = \e^B$, whence $B = 1$. Thus, $y = x^2 \e^x$.
\end{solution}

\begin{problem}
    $T_n(x)$ is a polynomial of degree $n$ in $x$ defined by $T_n(x) = \cos{n \arccos x}$ so that $T_n(\cos \t) = \cos{n \t}$.

    \begin{enumerate}
        \item Show that $T_2(x) = 2x^2 - 1$ and $T_3(x) = 4x^3 - 3x$.
        \item Show that $T_{n+1} (x) = 2x T_n (x) - T_{n-1} (x)$.
        \item Use the results in (a) and (b) to find $T_4(x)$.
    \end{enumerate}

    $U_n(x)$ is a polynomial of degree $n$ in $x$ defined by \[U_n(x) = \frac{\sin (n+1)\t}{\sin \t}\] where $x = \cos \t$.

    \begin{enumerate}
        \setcounter{enumi}{3}
        \item Show that \[\der{}{x} T_n(x) = nU_{n-1}(x).\]
        \item Show that \[\der{}{x} U_{n-1}(x) = \frac{xU_{n-1}(x) - n T_n(x)}{1 - x^2}.\]
        \item Deduce that $y = T_n(x)$ satisfies the differential equation \[\bp{1 - x^2} \der[2]{y}{x} - x\der{y}{x} + n^2 y = 0.\]
    \end{enumerate}
\end{problem}
\clearpage
\begin{solution}
    \begin{ppart}
        Since $T_2(\cos \t) = \cos 2\t = 2\cos^2 - 1$, it follows that $T_2(x) = 2x^2 - 1$. Similarly, since $T_3(\cos \t) = \cos 3\t = 4\cos^3 x - 3\cos x$, it follows that $T_3(x) = 4x^3 - 3x$.
    \end{ppart}
    \begin{ppart}
        Observe that
        \begin{align*}
            T_{n+1}(\cos \t) &= \cos (n+1)\t = \cos n\t \cos \t - \sin n\t \sin \t\\
            &= 2\cos n\t \cos \t - \bp{\cos n\t \cos \t + \sin n\t \sin \t}\\
            &= 2\cos n\t \cos \t - \cos (n-1)\t.
        \end{align*}
        Thus, $T_{n+1}(x) = 2x T_n(x) - T_{n-1}(x)$.
    \end{ppart}
    \begin{ppart}
        We have \[T_4(x) = 2xT_3(x) - T_2(x) = 2x\bp{4x^3 - 3x} - \bp{2x^2 - 1} = 8x^4 - 8x^2 + 1.\]
    \end{ppart}
    \begin{ppart}
        Since $x = \cos \t$, we have $\sin \t = \sqrt{1 - x^2}$. Hence, \[U_{n} (x) = \frac{\sin (n+1)\t}{\sin \t} = \frac{\sin{(n+1)\arccos x}}{\sqrt{1 - x^2}}.\] Thus, we have
        \begin{align*}
            \der{}{x} T_n (x) &= \der{}{x} \cos{n \arccos x}\\
            &= -\sin{n \arccos x} \bp{\frac{-n}{\sqrt{1 - x^2}}}\\
            &= n \frac{\sin{n \arccos x}}{\sqrt{1 -x^2}}\\
            &= n U_{n-1}(x).
        \end{align*}
    \end{ppart}
    \begin{ppart}
        We have
        \begin{align*}
            \der{}{x} U_{n-1}(x) &= \der{}{x} \frac{\sin{n\arccos x}}{\sqrt{1 - x^2}} \\
            &= \frac{1}{1 - x^2} \bs{\sqrt{1 - x^2} \bp{\frac{-n \cos{n \arccos x}}{\sqrt{1 - x^2}}} - \sin{n\arccos x} \bp{\frac{-x}{\sqrt{1 - x^2}}}}\\
            &= \frac{1}{1 - x^2} \bs{-n \cos{n \arccos x} + x \frac{\sin{n\arccos x}}{\sqrt{1 - x^2}} }\\
            &= \frac{-nT_n(x) + xU_{n-1}(x)}{1 - x^2}.
        \end{align*}
    \end{ppart}
    \begin{ppart}
        Note that $y = T_n(x)$ implies $y' = n U_{n-1}(x)$. Differentiating once more yields \[y'' = n \bp{\frac{xU_{n-1}(x)-nT_n(x)}{1 - x^2}} = \frac{nxU_{n-1}(x)-n^2T_n(x)}{1 - x^2} = \frac{x y' - n^2 y}{1 - x^2}.\] Rearranging, we obtain $\bp{1 - x^2} y'' - x y' + n^2 y = 0$.
    \end{ppart}
\end{solution}