\section{Self-Practice B4}

\begin{problem}
    Differentiate each of the following with respect to $x$, simplifying your answer.
    \begin{enumerate}
        \item $\frac{x^2 - 2x}{(x+2)^2}$,
        \item $x\bp{x^3 + 1}^{1/3}$,
        \item $\cot x \csc x$,
        \item $\bp{\sin^3 x} (\sin 3x)$,
        \item $\arctan \sqrt x$,
        \item $\arcsin \sqrt{1 - x^2}$,
        \item $y = \frac{\e^{2x}}{1 + \e^x}$,
        \item $y = \ln \frac4{x^2}$,
        \item $y = 3^x$.
    \end{enumerate}
\end{problem}
\begin{solution}
    \begin{ppart}
        We have \[\der{}{x} \frac{x^2 - 2x}{(x+2)^2} = \frac{\bp{x+2}^2 \bp{2x-2} - \bp{x^2 - 2x} \bs{2(x+2)}}{\bp{x+2}^4} = \frac{2\bp{3x-2}}{\bp{x+2}^3}.\]
    \end{ppart}
    \begin{ppart}
        We have \[\der{}{x} x\bp{x^3 + 1}^{1/3} = \bp{x^3 + 1}^{1/3} + x\bs{\frac13 \bp{x^3+1}^{-2/3} \cdot 3x^2} = \frac{2x^3 + 1}{\bp{x^3+1}^{2/3}}.\]
    \end{ppart}
    \begin{ppart}
        We have
        \begin{align*}
            \der{}{x} \cot x \csc x &= \bp{-\csc^2 x}\bp{\csc x} + \bp{\cot x}\bp{-\csc x \cot x}\\
            &= -\csc x \bp{\csc^2 x + \cot^2 x}\\
            &= \frac{1 + \cos^2 x}{\sin^3 x}.
        \end{align*}
    \end{ppart}
    \begin{ppart}
        We have
        \begin{align*}
            \der{}{x} \sin^3 x \sin 3x &= \bp{\sin^3 x}\bp{3\cos 3x} + \bp{3\sin^2 x \cos x}\bp{\sin 3x}\\
            &= 3\sin^2 x \bp{\sin x \cos 3x + \cos x \sin 3x}\\
            &= 3\sin^2 x \sin 4x.
        \end{align*}
    \end{ppart}
    \begin{ppart}
        We have \[\der{}{x} \arctan \sqrt{x} = \frac1{1 + \bp{\sqrt x}^2} \cdot \frac1{2 \sqrt x} = \frac1{2 \sqrt{x} \bp{1 + x}}.\]
    \end{ppart}
    \begin{ppart}
        We have \[\der{}{x} \arctan \sqrt{1 - x^2} = \frac1{\sqrt{1 - \bp{\sqrt{1-x^2}}^2}} \cdot \frac{-2x}{2\sqrt{1 - x^2}} = -\frac{x}{\abs{x} \sqrt{1 - x^2}}.\]
    \end{ppart}
    \begin{ppart}
        We have \[\der{y}{x} = \frac{\bp{1 + \e^x}\bp{2\e^{2x}} - \bp{\e^x}\bp{\e^{2x}}}{\bp{1 + \e^x}^2} = \frac{\e^{2x} \bp{2 + \e^x}}{\bp{1 + \e^x}^2}.\]
    \end{ppart}
    \begin{ppart}
        Note that $y = \ln{4/x^2} = \ln 4 - 2\ln x$. Hence, \[\der{y}{x} = -\frac{2}{x}.\]
    \end{ppart}
    \begin{ppart}
        Taking logarithms, we get $\ln y = x \ln 3$. Implicitly differentiating with respect to $x$, we obtain \[\frac1y \der{y}{x} = \ln 3 \implies \der{y}{x} = y \ln 3 = 3^x \ln 3.\]
    \end{ppart}
\end{solution}

\begin{problem}
    Find an expression for $\der{y}{x}$ in terms of $x$ and $y$.
    \begin{enumerate}
        \item $x^3 + y^3 + 3xy -1 = 0$,
        \item $y^x = x$.
    \end{enumerate}
\end{problem}
\begin{solution}
    \begin{ppart}
        Implicitly differentiating with respect to $x$, we obtain \[3x^2 + 3y^2 \der{y}{x} + 3x \der{y}{x} + 3y = 0 \implies \der{y}{x} = -\frac{x^2 + y}{x + y^2}.\]
    \end{ppart}
    \begin{ppart}
        Taking logarithms, we have $x \ln y = \ln x$. Implicitly differentiating with respect to $x$, \[x \bp{\frac1y \der{y}{x}} + \ln y = \frac1x \implies \der{y}{x} = \bp{\frac1x - \ln y} \frac{y}{x} = \frac{y \bp{1 - \ln x}}{x^2}.\]
    \end{ppart}
\end{solution}

\begin{problem}
    It is given that, at any point on the graph of $y = f(x)$, $\der{y}{x} = \sqrt{1 + y^3}$.
    \begin{enumerate}
        \item Show that $\der[2]{y}{x} = \frac32 y^2$.
        \item Find the expressions for $\der[3]{y}{x}$ and $\der[4]{y}{x}$ in terms of $y$ and $\der{y}{x}$.
    \end{enumerate}
\end{problem}
\begin{solution}
    \begin{ppart}
        Differentiating with respect to $x$, \[\der[2]{y}{x} = \frac{3y^2}{2\sqrt{1 + y^3}} \der{y}{x} = \frac{3y^2}{2\sqrt{1 + y^3}} \bp{\sqrt{1 + y^3}} = \frac{3y^2}{2}.\]
    \end{ppart}
    \begin{ppart}
        Differentiating once more with respect to $x$, we see that \[\der[3]{y}{x} = \frac{3}{2} \bp{2y} \der{y}{x} = 3y \der{y}{x}.\] Differentiating again, we have \[\der[4]{y}{x} = 3y \der[2]{y}{x} + 3\bp{\der{y}{x}}^2 = 3y\bp{\frac32 y^2} + 3\bp{\der{y}{x}}^2 = \frac{9y^3}{2} + 3\bp{\der{y}{x}}^2.\]
    \end{ppart}
\end{solution}
\clearpage

\begin{problem}
    Given that $y = \e^{\sqrt{1 + x}}$, show that \[4(1 + x) \der[2]{y}{x} + 2\der{y}{x} = y.\]
\end{problem}
\begin{solution}
    Note that \[\der{y}{x} = \e^{\sqrt{1 + x}} \frac1{2\sqrt{1 + x}} = \frac{y}{2\sqrt{1 + x}}.\] Differentiating once more, we find that \[\der[2]{y}{x} = \frac{\bp{2\sqrt{1 + x}}y' - \bp{1/\sqrt{1 + x} y}}{4\bp{1 + x}}.\] Rearranging, we get the desired result: \[4\bp{1 + x} \der[2]{y}{x} = 2\sqrt{1 + x} \der{y}{x} - \frac{y}{\sqrt{1 + x}} = y - 2\der{y}{x}.\]
\end{solution}

\begin{problem}
    \begin{enumerate}
        \item A curve has parametric equations $x = t/(1+t)$, $y = \ln \cos t$, where $t \neq -1, \pi/2$. Find $\derx{y}{x}$ in terms of $t$.
        \item A curve has equation $\arcsin y + x\e^y = 3x$. Find $\derx{y}{x}$ in terms of $x$ and $y$.
    \end{enumerate}
\end{problem}
\begin{solution}
    \begin{ppart}
        Note that \[\der{x}{t} = \frac{\bp{1 + t} - t}{\bp{1 + t}^2} = \frac1{(1 + t)^2} \quad \tand \quad \der{y}{t} = -\frac{\sin t}{\cos t} = -\tan t.\] Thus, \[\der{y}{x} = \frac{\derx{y}{t}}{\derx{x}{t}} = \frac{-\tan t}{(1+t)^{-2}} = -\bp{1 + t}^2 \tan t.\]
    \end{ppart}
    \begin{ppart}
        Implicitly differentiating with respect to $x$, \[\frac{y'}{\sqrt{1 - y^2}} + x \e^y y' + \e^y = 3 \implies \der{y}{x} = \frac{3 - \e^y}{(1 - y^2)^{-1/2} + x\e^y} = \frac{\bp{3 - \e^y} \sqrt{1 - y^2}}{1 + x\e^y \sqrt{1 - y^2}}.\]
    \end{ppart}
\end{solution}

\begin{problem}
    \begin{enumerate}
        \item Differentiate $\frac{x - 2x^3}{\ln x}$ with respect to $x$.
        \item Given that $0 < x < \frac\pi2$, show that $\der{}{x} \arcsin{\cos x} = k$, where $k$ is a real constant to be determined.
        \item Given that $\e^{xy} = \bp{1 + y^2}^2$, find $\der{y}{x}$ in terms of $x$ and $y$, simplifying your answer.
    \end{enumerate}
\end{problem}
\clearpage
\begin{solution}
    \begin{ppart}
        We have \[\der{}{x} \frac{x - 2x^3}{\ln x} = \frac{\ln x \bp{1 - 6x^2} - \bp{1/x} \bp{x - 2x^3}}{\ln^2 x} = \frac{\bp{1 - 6x^2}\ln x- 1 + 2x^2}{\ln^2 x}.\]
    \end{ppart}
    \begin{ppart}
        We have \[\der{}{x} \arcsin \cos x = -\frac{\sin x}{\sqrt{1 - \cos^2 x}} = -\frac{\sin x}{\sin x} = -1.\]
    \end{ppart}
    \begin{ppart}
        Taking logarithms, we have \[xy = 2 \ln{1 + y^2}.\] Implicitly differentiating with respect to $x$, \[xy' + y = 2\bp{\frac{2y \cdot y'}{1 + y^2}} \implies \der{y}{x} = \frac{y}{\frac{4y}{1+y^2} - x} = \frac{y\bp{1 + y^2}}{4y - x\bp{1 + y^2}}.\]
    \end{ppart}
\end{solution}

\begin{problem}
    It is given that $y = \ln \sin{\frac\pi4 + x}$. Show that \[\der[2]{y}{x} + \bp{\der{y}{x}}^2 + 1 = 0.\]
\end{problem}
\begin{solution}
    It suffices to show that \[\der[2]{y}{u} + \bp{\der{y}{u}}^2 + 1 = 0,\] where $u = \pi/4 + x$. Indeed, we have $y = \ln \sin u$, so \[\der{y}{u} = \frac{\cos u}{\sin u} = \cot u \quad \tand \quad \der[2]{y}{u} = -\csc^2 u,\] so \[\der[2]{y}{u} + \bp{\der{y}{u}}^2 + 1 = -\csc^2 u + \cot^2 u + 1 = -\csc^2 u + \csc^2 u = 0.\]
\end{solution}

\begin{problem}
    \begin{enumerate}
        \item Differentiate the following with respect to $x$, giving your answers as single fractions.
        \begin{enumerate}
            \item $\ln \frac{x}{\sqrt{1 - 2x}}$,
            \item $\frac1{\arccos{x^2}}$.
        \end{enumerate}
        \item The variables $x$ and $y$ are related by \[\e^{xy^2} = y \bp{x^2 + 2\e^x}.\] Find the value of $\der{y}{x}$ when $x = 0$ and $y = \frac12$.
    \end{enumerate}
\end{problem}
\begin{solution}
    \begin{ppart}
        \begin{psubpart}
            We have \[\der{}{x} \ln \frac{x}{\sqrt{1 - 2x}} = \frac{\sqrt{1-2x}}{x} \cdot \frac{\sqrt{1-2x} - x\bp{-\frac{2}{2\sqrt{1-2x}}}}{1 - 2x} = \frac{1-x}{x\bp{1 - 2x}}.\]
        \end{psubpart}
        \begin{psubpart}
            We have \[\der{}{x} \frac1{\arccos{x^2}} = \bp{-\frac{1}{\bs{\arccos{x^2}}^2}} \bp{-\frac1{\sqrt{1 - (x^2)^2}}}\bp{2x} = \frac{2x}{\sqrt{1 - x^4} \bs{\arccos{x^2}}^2}.\]
        \end{psubpart}
    \end{ppart}
    \begin{ppart}
        Implicitly differentiating with respect to $x$, we get \[\e^{xy^2} \bp{y^2 + 2xy\cdot y'} = y' \bp{x^2 + 2\e^x} + y\bp{2x + 2\e^x}.\] At $(0, 1/2)$, we have \[\frac14 = 2y' + 1 \implies y' = -\frac38.\]
    \end{ppart}
\end{solution}