\section{Assignment A10.3}

\begin{problem}
    \begin{enumerate}
        \item Solve $z^4 = -4 - 4\sqrt3 \i$, expressing your answers in the form $r\e^{\i\t}$, where $r > 0$ and $-\pi < \t \leq \pi$.
        \item Sketch the roots on an Argand diagram.
        \item Hence, solve $w^4 = -1 + \sqrt3 \i$, expressing your answers in a similar form.
    \end{enumerate}
\end{problem}
\begin{solution}
    \begin{ppart}
        Observe that $-4-4\sqrt3\i = 8\bp{-\frac12 - \frac{\sqrt3}2\i} = 8\e^{\i\frac43 \pi + 2k\pi \i}$ for all $k \in \ZZ$. Hence, \[z^4 = 8\e^{\i\frac43 \pi + 2k\pi \i} \implies z = 8^{\frac14} \e^{\i\frac13 \pi + \frac12 k\pi \i} = 2^{\frac34} \e^{\i \frac{2 + 3k}{6} \pi}.\] Taking $k = -2, -1, 0, 1$, we see that the roots are \[z_{-2} = 2^{\frac34} \e^{-\i\frac23\pi}, \quad z_{-1} = 2^{\frac34} \e^{-\i\frac16\pi}, \quad z_{0} = 2^{\frac34} \e^{\i\frac13\pi}, \quad z_{1} = 2^{\frac34} \e^{\i\frac56\pi}.\]
    \end{ppart}
    \begin{ppart}
        \begin{center}\tikzsetnextfilename{72}
            \begin{tikzpicture}[trim axis left, trim axis right]
                \begin{axis}[
                    domain = 0:10,
                    samples = 101,
                    axis y line=middle,
                    axis x line=middle,
                    xtick = \empty,
                    ytick = \empty,
                    xmax=2.4,
                    xmin=-2.4,
                    ymin=-2.1,
                    ymax=2.1,
                    xlabel = {$\Re$},
                    ylabel = {$\Im$},
                    legend cell align={left},
                    legend pos=outer north east,
                    after end axis/.code={
                        \path (axis cs:0,0) 
                            node [anchor=north east] {$O$};
                        }
                    ]
        
                    \coordinate (R) at (10,0);
                    \coordinate[label=below left:$z_{-2}$] (Z-2) at (-0.84089, -1.4565);
                    \coordinate[label=right:$z_{-1}$] (Z-1) at (1.4565, -0.84089);
                    \coordinate[label=right:$z_{0}$] (Z0) at (0.84089, 1.4565);
                    \coordinate[label=left:$z_{1}$] (Z1) at (-1.4565, 0.84089);
                    \coordinate (O) at (0, 0);

                    \draw[dashed] (O) circle[radius=8^0.25];

                    \node[rotate=60, anchor=south] at (0.42, 0.7) {$2^{\frac34}$};
            
                    \draw (O) -- (Z-2);
                    \draw (O) -- (Z-1);
                    \draw (O) -- (Z0);
                    \draw (O) -- (Z1);
            
                    \fill (Z-2) circle[radius=2.5pt];
                    \fill (Z-1) circle[radius=2.5pt];
                    \fill (Z0) circle[radius=2.5pt];
                    \fill (Z1) circle[radius=2.5pt];
                    \draw pic [draw, angle radius=5mm, ""] {angle = R--O--Z0};

                    \node at (0.45, 0.24) {$\frac\pi3$};

                    \draw pic [draw, angle radius=3mm, "$\cdot$"] {right angle = Z0--O--Z1};
                    \draw pic [draw, angle radius=3mm, "$\cdot$"] {right angle = Z-1--O--Z0};
                    \draw pic [draw, angle radius=3mm, "$\cdot$"] {right angle = Z-2--O--Z-1};
                    \draw pic [draw, angle radius=3mm, "$\cdot$"] {right angle = Z1--O--Z-2};
                \end{axis}
            \end{tikzpicture}
        \end{center}
    \end{ppart}
    \begin{ppart}
        Observe that $w^{4} = -1 + \sqrt3 \i = \frac14 (-4 + 4\sqrt3 \i) = 2^{-2} (z\conj)^4$. Hence, $w = 2^{-1/2} z\conj$. Thus, the roots are \[w_{-2} = 2^{\frac14} \e^{\i\frac23\pi}, \quad w_{-1} = 2^{\frac14} \e^{\i\frac16\pi}, \quad w_{0} = 2^{\frac14} \e^{-\i\frac13\pi}, \quad w_{1} = 2^{\frac14} \e^{-\i\frac56\pi}.\]
    \end{ppart}
\end{solution}

\begin{problem}
    Let
    \begin{align*}
        C &= 1 - \binom{2n}{1} \cos \t + \binom{2n}{2} \cos 2\t - \binom{2n}{3} \cos 3\t + \ldots + \cos 2n\t\\
        S &= - \binom{2n}{1} \sin \t + \binom{2n}{2} \sin 2\t - \binom{2n}{3} \sin 3\t + \ldots + \sin 2n\t
    \end{align*}
    where $n$ is a positive integer.

    Show that $C = (-4)^n \cos{n\t} \sin[2n]{\t/2}$, and find the corresponding expression for $S$.
\end{problem}
\begin{solution}
    Clearly, \[C = \sum_{k = 0}^{2n} \binom{2n}{k} (-1)^k \cos k\t, \quad S = \sum_{k = 0}^{2n} \binom{2n}{k} (-1)^k  \sin k\t.\] Hence,
    \begin{align*}
        C + \i S &= \sum_{k = 0}^{2n} \binom{2n}{k} (-1)^k (\cos k\t + \i\sin k\t)\\
        &= \sum_{k = 0}^{2n} \binom{2n}{k} (-\e^{\i\t})^k = \bp{1 - \e^{\i\t}}^{2n}\\
        &= \bp{\e^{\i\t/2}}^{2n} \bp{\e^{-\i\t/2} - \e^{\i\t/2}}^{2n}\\
        &= \e^{\i n \t} \bp{2\i \sin \frac\t2}^{2n}\\
        &= \e^{\i n \t} (-4)^n \sin^{2n} \frac\t2\\
        &= (\cos n\t + \i\sin n\t) (-4)^n \sin^{2n} \frac\t2.
    \end{align*}

    Comparing real and imaginary parts, we have \[C = (-4)^n \cos{n\t} \sin^{2n} \frac\t2, \quad S = (-4)^n \sin{n\t} \sin^{2n} \frac\t2.\]
\end{solution}

\begin{problem}
    Given that $z = \cos\t + \i\sin\t$, show that
    \begin{enumerate}
        \item $z - 1/z = 2\i\sin\t$,
        \item $z^n + z^{-n} = 2\cos n\t$.
    \end{enumerate}

    Hence, show that \[\sin^6 \t = \frac1{32} (10 - 15\cos2\t + 6\cos4\t - \cos6\t)\] Find a similar expression for $\cos^6 \t$, and hence express $\cos^6 \t - \sin^6 \t$ in the form $a\cos2\t + b\cos6\t$.
\end{problem}
\begin{solution}
    \begin{ppart}
        Note that \[z - \frac1z = z - z^{-1} = \e^{\i\t} - \e^{-\i\t} = [\cos \t + \i\sin \t] - [\cos{-\t} + \i\sin{-\t}] = 2\i\sin \t.\]
    \end{ppart}
    \begin{ppart}
        Note that \[z^n + z^{-n} = \e^{\i n\t} + e^{-\i n\t} = [\cos n\t + \i\sin n\t] + [\cos{-n\t} + \i\sin{n\t}] = 2\cos n\t.\]
    \end{ppart}

    Observe that
    \begin{align*}
        \sin^6 \t &= \frac1{(2\i)^6} (2\i \sin \t)^6 = -\frac1{64} (z - z^{-1})^6\\
        &= -\frac1{64} \bp{z^6 - 6 z^4 + 15 z^2 - 20 + 15 z^{-2} - 6 z^{-4} + z^{-6}}\\
        &= -\frac1{32} \bs{-\frac{20}2 + 15\bp{\frac{z^2 + z^{-2}}2} -6\bp{\frac{z^4 + z^{-4}}2} + \bp{\frac{z^6 + z^{-6}}2}}\\
        &= \frac1{32} \bp{10 - 15\cos2\t + 6\cos4\t - \cos6\t}.
    \end{align*}

    Similarly, 
    \begin{align*}
        \cos^6 \t &= \frac1{2^6} (2\cos\t)^6 = \frac1{64} (z + z^{-1})^6\\
        &= \frac1{64} \bs{z^6 + 6 z^4 + 15 z^2 + 20 + 15 z^{-2} + 6 z^{-4} + z^{-6}}\\
        &= \frac1{32} \bs{\frac{20}2 + 15\bp{\frac{z^2 + z^{-2}}2} + 6\bp{\frac{z^4 + z^{-4}}2} + \bp{\frac{z^6 + z^{-6}}2}}\\
        &= \frac1{32} \bp{10 + 15\cos2\t + 6\cos4\t + \cos6\t}.
    \end{align*}

    Hence, \[\cos^6 \t - \sin^6 \t = \frac1{32} (30 \cos 2\t + 2\cos 6\t) = \frac{15}{16} \cos 2\t + \frac1{16} \cos 6\t,\] whence $a = 15/16$ and $b = 1/16$.
\end{solution}