\section{Self-Practice A10.3}

\begin{problem}
    Express $\frac{\cot \t + \i}{\cot \t - \i}$ in the exponential form. Hence, show that one of the roots of the equation \[z^4 = \frac{\sqrt3 + \i}{\sqrt3 - \i}\] is $\e^{\i \pi/12}$, and find three more roots in the exponential form.
\end{problem}
\begin{solution}
    Note that \[\frac{\cot \t + \i}{\cot \t - \i} = \frac{\cos \t + \i \sin \t}{\cos \t - \i \sin \t} = \frac{\e^{\i\t}}{\e^{-\i\t}} = \e^{2\i \t}.\]

    Note that $\cot \t = \sqrt{3} \implies \t = \pi/6$, so \[z^4 = \frac{\sqrt3 + \i}{\sqrt3 - \i} = \e^{2\i \pi/6} = \e^{\i \pi (1/3 + 2k)},\] where $k \in \ZZ$. Taking fourth roots, \[z = \e^{\i \pi (1/12 + k/2)}.\] Taking $k = 0, 1, 2, 3$, we see that the four roots are \[z = \e^{\i \pi /12}, \, \e^{7\i \pi/12}, \, \e^{13\i \pi/12}, \, \e^{19\i \pi/12}.\]
\end{solution}

\begin{problem}
    Find the cube roots of the complex number $1 + \i \sqrt3$. Give your answers exactly, in the form $r\e^{\i \t}$. Hence, solve the equation $z^6 - 2z^3 + 4 = 0$. Give your answers exactly, in the form $r\e^{\i \t}$.
\end{problem}
\begin{solution}
    Consider \[z^3 = 1 + \i \sqrt{3} = 2 \e^{\i \pi /3} = 2\e^{\i \pi (1/3 + 2k)},\] where $k \in \ZZ$. Taking roots, \[z = 2^{1/3} \e^{\i \pi (1/9 + 2k/3)}.\] Taking $k = -1, 0, 1$, the cube roots of $1 + \i \sqrt{3}$ are \[z = 2^{1/3} \e^{-8\i \pi /9}, 2^{1/3} \e^{\i \pi / 9}, 2^{1/3} \e^{7\i \pi/9}.\] Consider $z^6 - 2z^3 + 4 = 0$. Then \[z^3 = 1 \pm \sqrt{3}.\] From the positive branch, we get the aforementioned roots. Since the coefficients of the sextic are all real, by the conjugate root theorem, the six roots are \[z = 2^{1/3} \e^{-8 \i \pi / 9}, \, 2^{1/3} \e^{-7\i \pi/9}, \, 2^{1/3} \e^{-\i \pi /9}, \, 2^{1/3} \e^{\i \pi / 9}, \, 2^{1/3} \e^{7\i \pi/9}, \, 2^{1/3} \e^{8\i \pi /9}.\]
\end{solution}

\begin{problem}
    Express $8\bp{\sqrt3 - \i}$ in the form $r\bp{\cos \t + \i \sin \t}$, where $r > 0$ and $-\pi \leq \t \leq \pi$, giving $\t$ in terms of $\pi$. Hence, obtain the roots of the equation $z^4 = 8\bp{\sqrt3 - \i}$ in the same form.
\end{problem}
\begin{solution}
    Note that \[8\bp{\sqrt 3 - \i} = 16 \bp{\frac{\sqrt3}{2} - \frac12 \i} = 16 \bs{\cos{-\frac\pi6} + \i \sin{-\frac\pi6}} = 16 \e^{-\i \pi/6}.\] 

    We are given \[z^4 = 8\bp{\sqrt3 - \i} = 16 \e^{-\i \pi/6} = 16\e^{\i \pi (-1/6 + 2k)},\] for $k \in \ZZ$. Taking roots, \[z = 2 \e^{\i \pi (-1/24 + k/2)}.\] Taking $k = -1, 0, 1, 2$, the roots are \[z = 2\e^{-13\i\pi/24}, \, 2\e^{-\i\pi/24}, \, 2\e^{11\i\pi/24}, \, 2\e^{23\i\pi/24}.\]
\end{solution}

\begin{problem}
    Write down, in any form, the five complex numbers which satisfy the equation $z^5 - 1 = 0$. Hence, show that the five complex numbers which satisfy the equation \[\bp{\frac{2w + 1}{w}}^5 = 1\] are \[\frac{-2 + \cos{\frac25 \pi k} - \i \sin{\frac25 \pi k}}{5 - 4 \cos{\frac25 \pi k}},\] where $k = 0, 1, 2, 3, 4$.
\end{problem}
\begin{solution}
    The fifth roots of unity are given by \[z = \e^{2k \i \pi /5},\] where $k = 0, 1, 2, 3, 4$.

    We have \[\frac{2w + 1}{w} = \e^{2k \i \pi /5} \implies w = \frac1{\e^{2k \i \pi /5} - 2} = \frac{\e^{-2k \i \pi /5} - 2}{\abs{\e^{2k \i \pi /5} - 2}^2}.\] Note that \[\abs{\e^{2k \i \pi /5} - 2}^2 = \bp{\e^{2k \i \pi /5} - 2}\bp{\e^{-2k \i \pi /5} - 2} = 1 - 2\bp{2\cos \frac{2k\pi}{5}} + 4 = 5 - 4\cos \frac{2k\pi}5.\] Thus, \[w = \frac{-2 + \cos{\frac25 \pi k} - \i \sin{\frac25 \pi k}}{5 - 4 \cos{\frac25 \pi k}}\] for $k = 0, 1, 2, 3, 4$.
\end{solution}

\begin{problem}
    \begin{enumerate}
        \item Show that, for all complex numbers $z$ and all real numbers $\a$, \[\bp{z - \e^{\i \a}} \bp{z - \e^{-\i \a}} = z^2 - 2z\cos \a + 1.\]
        \item Write down, in any form, the seven complex numbers which satisfy the equation $z^7 - 1 = 0$.
        \item Hence, show that, for all complex numbers $z$, \[z^7 - 1 = (z-1)\bs{z^2 - 2z\cos \frac{2\pi}7 + 1}\bs{z^2 - 2z\cos \frac{4\pi}7 + 1}\bs{z^2 - 2z\cos \frac{6\pi}7 + 1}.\]
    \end{enumerate}
\end{problem}
\begin{solution}
    \begin{ppart}
        We have \[\bp{z - \e^{\i \a}} \bp{z - \e^{-\i \a}} = z^2 - \bp{\e^{\i \a} + \e^{-\i \a}} z + 1 = z^2 - 2z\cos \a + 1.\]
    \end{ppart}
    \begin{ppart}
        The seventh roots of unity are \[z = \e^{2k\i \pi/7}\] where $k = -3, -2, -1, 0, 1, 2, 3$.
    \end{ppart}
    \begin{ppart}
        Let $P_k = z - \e^{2k\i \pi/7}$. Observe that \[P_{k}P_{-k} = \bp{z - \e^{2k\i \pi/7}}\bp{z - \e^{2k\i \pi/7}} = z^2 - 2z\cos \frac{2k \pi}{7} + 1.\] Hence,
        \begin{align*}
            z^7 - 1 &= P_0 \bp{P_1 P_{-1}} \bp{P_2 P_{-2}} \bp{P_{3} P_{-3}}\\
            &= (z-1)\bs{z^2 - 2z\cos \frac{2\pi}7 + 1}\bs{z^2 - 2z\cos \frac{4\pi}7 + 1}\bs{z^2 - 2z\cos \frac{6\pi}7 + 1}.
        \end{align*}
    \end{ppart}
\end{solution}

\begin{problem}
    Use De Moivre's theorem to show that \[\cos 6\t = 32 \cos^6 \t - 48 \cos^4 \t + 18\cos^2 \t - 1.\] Deduce that, for all $\t$, \[0 \leq \cos^6 \t - \frac32 \cos^4 \t + \frac9{16} \cos^2 \t \leq \frac1{16}.\]
\end{problem}
\begin{solution}
    Let $c = \cos \t$ and $s = \sin \t$. Then 
    \begin{align*}
        \cos 6\t &= \Re \e^{6\i \t} = \Re \bp{c + \i s}^6\\
        &= \binom{6}{0} c^6 - \binom{6}{2} c^4 s^2 + \binom{6}{4} c^2 s^4 - \binom{6}{6} s^6\\
        &= c^6 - 15 c^4 \bp{1-c^2} + 15 c^2 \bp{1-c^2}^2 - \bp{1-c^2}^3\\
        &= c^6 - 15 c^4 \bp{1 - c^2} + 15 c^2 \bp{1 - 2c^2 + c^4} - \bp{1 - 3c^2 + 3c^4 - c^6}\\
        &= 32c^6 - 48c^4 + 18c^2 - 1\\
        &= 32 \cos^6 \t - 48 \cos^4 \t + 18\cos^2 \t - 1.
    \end{align*}

    Observe that \[-\frac1{32} \leq \frac{\cos 6\t}{32} = \cos^6 \t - \frac32 \cos^4 \t + \frac9{16} \cos^2 \t - \frac1{32} \leq \frac1{32},\] so \[0 \leq \cos^6 \t - \frac32 \cos^4 \t + \frac9{16} \cos^2 \t \leq \frac1{16}.\]
\end{solution}

\begin{problem}
    Show that for $z \neq -1$, \[z - z^2 + z^3 - \dots + z^7 = \frac{z + z^8}{1 + z}.\] Hence, by substituting $z = \e^{\i \t}$, show that \[\sum_{k=1}^7 (-1)^{k-1} \sin k\t = \frac{\sin 4\t \cos \frac72 \t}{\cos \frac12 \t},\] where $\t$ is not an odd multiple of $\pi$.
\end{problem}
\begin{solution}
    Observe that $z - z^2 + z^3 - \dots + z^7$ is a geometric series with common ratio $-z$, so it evaluates to \[z - z^2 + z^3 - \dots + z^7 = z\bp{\frac{1 - (-z)^7}{1 - (-z)}} = \frac{z - z^8}{1 + z},\] with the condition $z \neq -1$.

    We have
    \begin{align*}
        \sum_{k=1}^7 (-1)^{k-1} \sin k\t &= \sum_{k=1}^7 (-1)^{k-1} \Im z^k = \Im \sum_{k=1}^7 (-1)^{k-1} z^k = \Im \frac{z + z^8}{1 + z}\\
        &= \Im \frac{z^{9/2} \bp{z^{7/2} + z^{-7/2}}}{z^{1/2} \bp{z^{1/2} + z^{-1/2}}} = \frac{2\cos{\frac72 \t}}{2\cos{\frac12 \t}} \Im z^4 = \frac{\cos{\frac72 \t} \sin 4\t}{\cos \frac12 \t}.
    \end{align*}
    Note that $z = \e^{\i \t} \neq -1 = \e^{\i \pi (2k + 1))}$ for $k \in \ZZ$, so $\t \neq (2k+1)\pi$, i.e. $\t$ cannot be an odd multiple of $\pi$.
\end{solution}