\section{An Introduction to the Mathematical Vernacular}

\begin{problem}
    Prove that the sum of even and even is even.
\end{problem}
\begin{proof}
    Let $a$ and $b$ be even. By definition, there exists $a', b' \in \ZZ$ such that $a = 2a'$ and $b = 2b'$. Thus, $a + b = 2a' + 2b' = 2\bp{a' + b'}$. Since $a' + b'$ is an integer, by definition, $a + b$ is even. Hence, the sum of even and even is even.
\end{proof}

\begin{problem}
    Prove that the sum of even and odd is odd.
\end{problem}
\begin{proof}
    Let $a$ be even and let $b$ be odd. By definition, there exists $a', b' \in \ZZ$ such that $a = 2a'$ and $b = 2b' + 1$. Thus, $a + b = 2a' + \bp{2b' + 1} = 2\bp{a' + b'} + 1$. Since $a' + b'$ is an integer, by definition, $a + b$ is odd. Hence, the sum of even and odd is odd.
\end{proof}

\begin{problem}
    Prove that the sum of odd and odd is even.
\end{problem}
\begin{proof}
    Let $a$ and $b$ be odd. By definition, there exists $a', b' \in \ZZ$ such that $a = 2a' + 1$ and $b = 2b' + 1$. Thus, $a + b = 2\bp{a' + 1} + 2\bp{b' + 1} = 2\bp{a' + b' + 2}$. Since $a' + b' + 2$ is an integer, by definition, $a + b$ is even. Hence, the sum of odd and odd is even.
\end{proof}