\section{Assignment A10.1}

\begin{problem}
    The complex number $w$ is such that $w w\conj + 2w = 3 + 4\i$, where $w\conj$ is the complex conjugate of $w$. Find $w$ in the form $a + \i b$, where $a$ and $b$ are real.
\end{problem}
\begin{solution}
    Note $w w\conj = \bp{\Re w}^2 + \bp{\Im w}^2 \in \RR$.

    Taking the imaginary part of the given equation, \[\Im{ww\conj + 2w} = \Im{3 + 4i} \implies 2 \Im w = 4 \implies \Im w = 2.\] Taking the real part of the given equation,
    \begin{gather*}
        \Re{ww\conj + 2w} = \Re{3 + 4i} \implies \bs{\bp{\Re w}^2 + \bp{\Im w}^2} + 2\Re w = 3\\
        \implies \bp{\Re w}^2 + 2\Re {w} + 1 = 0 \implies \bp{\Re w + 1}^2 = 0 \implies \Re{w} = -1.
    \end{gather*}
    Hence, $w = -1 + 2\i$.
\end{solution}

\begin{problem}
    Express $(3 - \i)^2$ in the form $a + \i b$.

    Hence, or otherwise, find the roots of the equation $(z+\i)^2 = -8+6\i$.
\end{problem}
\begin{solution}
    We have \[(3 - \i)^2 = 3^2 - 6 \i + \i^2 = 8 - 6\i.\]

    Consider $(z+\i)^2 = -8+6\i$. Note that $-(z+\i)^2 = (\i z - 1)^2$.
    \begin{gather*}
        (z+\i)^2 = -8 + 6\i \implies (\i z - 1)^2 = 8 - 6\i \implies \i z - 1 = \pm (3 - \i)\\
        \implies z = \frac1\i (1 \pm (3 - \i)) = -\i(1 \pm (3 - \i)) = -1-4\i \lor 1 + 2\i.
    \end{gather*}
\end{solution}

\begin{problem}
    \begin{enumerate}
        \item It is given that $z_1 = 1 + \sqrt3 \i$. Find the value of $z_1^3$, showing clearly how you obtain your answer.
        \item Given that $1 + \sqrt3 \i$ is a root of the equation \[2z^3 + az^2 + bz + 4 = 0\] find the values of the real numbers $a$ and $b$. Hence, solve the above equation.
    \end{enumerate}
\end{problem}
\begin{solution}
    \begin{ppart}
        We have \[z_1^3 = \bp{1 + \sqrt3 \i}^3 = 1 + 3\bp{\sqrt3 \i} + 3\bp{\sqrt3 \i}^2 + \bp{\sqrt3 \i}^3 = 1 + 3\sqrt 3 \i - 9 - 3\sqrt3 \i = -8.\]
    \end{ppart}
    \begin{ppart}
        Since $1 + \sqrt3\i$ is a root of the given equation, we have
        \begin{gather*}
            2\bp{1 + \sqrt3\i}^3 + a\bp{1 + \sqrt3\i}^2 + b\bp{1 + \sqrt3 \i} + 4 = 0\\
            \implies -16 + a\bp{-2 + 2\sqrt3 \i} + b\bp{1 + \sqrt3\i} + 4 = 0 \implies (-2a + b) + \sqrt3 (2a + b) \i = 12.
        \end{gather*}
        Comparing real and imaginary parts, we obtain $-2a + b = 12$ and $2a + b = 0$, whence $a = -3$ and $b = 6$.

        Since the coefficients of $2z^3 + az^2 + bz + 4$ are all real, the second root is $(1 + \sqrt3\i)\conj = 1 - \sqrt3 \i$. Let the third root be $\a$. By Vieta's formula, \[(1 + \sqrt3\i)(1 - \sqrt3\i)\a = -\frac42 \implies 4\a = -2 \implies \a = -\frac12.\] The roots of the equation are hence $1 + \sqrt3\i$, $1 - \sqrt3\i$ and $-\frac12$.
    \end{ppart}
\end{solution}

\begin{problem}
    The complex number $z$ is such that $az^2 + bz + a = 0$ where $a$ and $b$ are real constants. It is given that $z = z_0$ is a solution to this equation where $\Im{z_0} \neq 0$.

    \begin{enumerate}
        \item Verify that $z = \frac1{z_0}$ is the other solution. Hence, show that $\abs{z_0} = 1$.
    \end{enumerate}

    Take $\Im{z_0} = 1/2$ for the rest of the question.

    \begin{enumerate}
        \setcounter{enumi}{1}
        \item Find the possible complex numbers for $z_0$.
        \item If $\Re{z_0} > 0$, find $b$ in terms of $a$.
    \end{enumerate}
\end{problem}
\begin{solution}
    \begin{ppart}
        \begin{equation*}
            a \bp{\frac1{z_0}}^2 + b\bp{\frac1{z_0}} + a = \bp{\frac1{z_0}}^2 \bp{a + bz_0 + az_0^2} = 0
        \end{equation*}
        Hence, $z = 1/z_0$ is a root of the given equation.

        Since $a, b \in \RR$, by the conjugate root theorem, $z_0\conj = 1/z_0$. Hence, \[z_0 z_0\conj = 1 \implies \Re{z_0}^2 + \Im{z_0}^2 = \abs{z_0}^2 = 1 \implies \abs{z_0} = 1.\]
    \end{ppart}
    \begin{ppart}
        Let $z_0 = x + \frac12\i$. Then \[\abs{x + \frac12 i} = 1 \implies x^2 + \bp{\frac12}^2 = 1^2 \implies x^2 = \frac34 \implies x = \pm\frac{\sqrt3}2.\] Hence, $z_0 = \frac{\sqrt3}2 + \frac12\i$ or $z_0 = -\frac{\sqrt3}2 + \frac12\i$.
    \end{ppart}
    \begin{ppart}
        Since $\Re{z_0} > 0$, we have $z_0 = \frac{\sqrt3}2 + \frac12\i$. By Vieta's formula, \[-\frac{b}{a} = z_0 + \frac1{z_0} = z_0 + z_0\conj = 2 \Re{z_0} = \sqrt3 \implies b = -\sqrt3 a.\]
    \end{ppart}
\end{solution}